src/bva/Bva_checker.v
@@ -767,8 +767,12 @@ Fixpoint check_symopp (bs1 bs2 bsres : list _lit) (bvop: binop)  :=
    end.
 
    Definition check_extract (bs bsres: list _lit) (i j: N) : bool :=
-     if (forallb2 eq_carry_lit (lit_to_carry (extract_lit bs (nat_of_N i) (nat_of_N j))) bsres)
-    then true else false.
+     if (N.ltb (N.of_nat (length bs)) j) 
+     then false
+     else
+       if (forallb2 eq_carry_lit (lit_to_carry (extract_lit bs (nat_of_N i) (nat_of_N j))) bsres)
+       then true
+       else false.
 
   Definition check_extract3 (bs bsres: list _lit) (i j: N) : bool :=
     forallb2 (fun l1 l2 => l1 == l2) (extract_lit bs (nat_of_N i) (nat_of_N j)) bsres.
@@ -795,7 +799,6 @@ Fixpoint check_symopp (bs1 bs2 bsres : list _lit) (bvop: binop)  :=
         end
    end.
 
-
   Definition check_bbExtract pos lres :=
     match S.get s pos with
       | l1::nil =>
@@ -804,10 +807,11 @@ Fixpoint check_symopp (bs1 bs2 bsres : list _lit) (bvop: binop)  :=
             | FbbT a1 bs, FbbT a bsres =>
               match get_atom a with
 
-                | Auop (UO_BVextr n i j H0 H1) a1' =>
+                | Auop (UO_BVextr i n0 n1) a1' =>
                   if ((a1 == a1') (* || ((a1 == a2') && (a2 == a1')) *) )
-                       && (check_extract bs bsres i j)
-                       && (N.of_nat (length bs) =? n)%N
+                       && (check_extract bs bsres i (n0 + i))
+                       && (N.of_nat (length bs) =? n1)%N
+                       && (N.leb (n0 + i) n1)
                   then lres::nil
                   else C._true
 
@@ -1315,7 +1319,7 @@ Proof. intros a bs.
          intro H3. rewrite H3 in H0. now contradict H0.
          intros n0 Hn. rewrite Hn in H0. now contradict H0.
          intros n0 Hn. rewrite Hn in H0. now contradict H0.
-         intros n0 i3 j H2 H3 Heq. rewrite Heq in H0. now contradict H0.
+         intros i3 n0 n1 Heq. rewrite Heq in H0. now contradict H0.
          intros n0 i3 Heq. rewrite Heq in H0. now contradict H0.
          intros n0 i3 Heq. rewrite Heq in H0. now contradict H0. 
          intros b0 i2 i3 Heq. rewrite Heq in H0. now contradict H0.
@@ -7026,46 +7030,83 @@ Proof. intro a.
          now rewrite IHa.
 Qed.
 
-Lemma extract_interp_main: forall bs1 bsres (n i j: N) (H0: (n >= j)%N) (H1: (j >= i)%N),
-                  check_extract bs1 bsres i j = true ->
-                  @RAWBITVECTOR_LIST.bv_extr n i j H0 H1 
+Lemma extract_interp_main: forall bs1 bsres (i n0: N),
+                  check_extract bs1 bsres i (n0 + i) = true ->
+                  @RAWBITVECTOR_LIST.bv_extr i n0 (N.of_nat (length bs1)) 
                     (map (Lit.interp rho) bs1) = map (Lit.interp rho) bsres.
 Proof. intro bs1.
        induction bs1 as [ | xbs1 xsbs1 IHbs1].
        - intros. simpl.
          unfold check_extract in H. simpl in H.
-         case_eq bsres. intros. simpl.
          unfold RAWBITVECTOR_LIST.bv_extr.
-         now simpl.
-         intros. rewrite H2 in H.
-         now contradict H.
+          case_eq (nat_of_N i).
+          intros. simpl.
+          case_eq (nat_of_N n0).
+          intros. simpl.
+         case_eq ((0 <? n0 + i)%N); intros.
+          rewrite H2 in H. now contradict H.
+          rewrite H2 in H.
+         case_eq bsres. intros. now simpl.
+          intros. rewrite H3 in H. now contradict H.
+          intros.
+          case_eq bsres. intros.
+          admit (****).
+          intros. rewrite H2 in H.
+          admit (****).
+          intros.
+          admit (****).
        - intros. unfold check_extract in H.
+         case_eq ((N.of_nat (Datatypes.length (xbs1 :: xsbs1)) <? n0 + i)%N).
+         intros. rewrite H0 in H. now contradict H.
+         intros. rewrite H0 in H.         
          case_eq (
           forallb2 eq_carry_lit
           (lit_to_carry
           (extract_lit (xbs1 :: xsbs1) 
-          (N.to_nat i) (N.to_nat j))) bsres); intros.
-         apply prop_eq_carry_lit2 in H2.
-         rewrite prop_interp_carry3 in H2.
-         simpl in H2. simpl.
+          (N.to_nat i) (N.to_nat (n0 + i)))) bsres); intros.
+         apply prop_eq_carry_lit2 in H1.
+         rewrite prop_interp_carry3 in H1.
+         simpl in H1. simpl.
 
          unfold RAWBITVECTOR_LIST.bv_extr in *.
          simpl in *.
-         case_eq (N.to_nat i); intros; rewrite H3 in H2.
-         case_eq (N.to_nat j); intros; rewrite H4 in H2.
-         rewrite <- H2. easy.
-         simpl in H2.
-         rewrite <- H2. simpl. apply f_equal.
+         case_eq (N.to_nat i); intros; rewrite H2 in H1.
+         case_eq (N.to_nat (n0 + i)); intros; rewrite H3 in H1.
+         rewrite <- H1. rewrite H0. easy.
+         rewrite H0.        
+
+         simpl in H1.
+         rewrite <- H1. simpl. apply f_equal.
          
          now rewrite extract_interp_zero.
          
-         case_eq (N.to_nat j); intros; rewrite H4 in H2.
-         rewrite <- H2. easy.
+         case_eq (N.to_nat (n0 + i)); intros; rewrite H3 in H1.
+         rewrite H0.
+         rewrite <- H1. easy.
          
+         rewrite H0.
          now rewrite extract_interp_all.
          
-         rewrite H2 in H. now contradict H.
-Qed.
+         rewrite H1 in H. now contradict H.
+Admitted.
+
+  Lemma Npos_dist: forall p p0: positive, (Npos (p + p0))%N = (Npos p + Npos p0)%N.
+  Proof. intros. case p in *; case p0 in *; easy. Qed.
+
+  Lemma not_ltb2: forall (n0 n1 i: N), (n1 >= n0 + i)%N -> (n1 <? n0 + i)%N = false.
+  Proof. intro n0.
+         induction n0.
+         intros. simpl in *.
+         now apply N.ltb_nlt in H.
+
+         intros. simpl.
+         case_eq i.
+         intros. subst. simpl in H.
+         now apply N.ltb_nlt in H.
+         intros. subst.
+         apply N.ltb_nlt in H.
+         now rewrite Npos_dist.
+  Qed.
 
 Lemma valid_check_bbExtract pos lres : C.valid rho (check_bbExtract pos lres).
 Proof.
@@ -7081,7 +7122,8 @@ Proof.
       (* BVextract *)
     - case_eq ((a1 == a1')); simpl; intros Heq7; try (now apply C.interp_true).
         case_eq (
-            check_extract bs1 bsres i j && (N.of_nat (Datatypes.length bs1) =? n)%N
+          check_extract bs1 bsres i (n0 + i) &&
+          (N.of_nat (Datatypes.length bs1) =? n1)%N && (n0 + i <=? n1)%N
         ); simpl; intros Heq8; try (now apply C.interp_true).
 
         unfold C.valid. simpl. rewrite orb_false_r.
@@ -7097,14 +7139,14 @@ Proof.
         pose proof (H a). 
         assert (a < PArray.length t_atom).
         { apply PArray.get_not_default_lt. rewrite def_t_atom. rewrite Heq6. easy. }
-        specialize (@H2 H3). rewrite Heq6 in H2. simpl in H2.
-        rewrite !andb_true_iff in H2. destruct H2.
+        specialize (@H0 H1). rewrite Heq6 in H0. simpl in H0.
+        rewrite !andb_true_iff in H0. destruct H0.
 
-        unfold get_type' in H2. unfold v_type in H2.
+        unfold get_type' in H0. unfold v_type in H0.
         case_eq (t_interp .[ a]).
-        intros v_typea v_vala Htia. rewrite Htia in H2.
-        case_eq (v_typea);  intros; rewrite H5 in H2; try (now contradict H2).
-        rename H2 into Hv.
+        intros v_typea v_vala Htia. rewrite Htia in H0.
+        case_eq (v_typea);  intros; rewrite H3 in H0; try (now contradict H2).
+        rename H0 into Hv.
 
         generalize (Hs pos). intros HSp. unfold C.valid in HSp. rewrite Heq1 in HSp.
         unfold C.interp in HSp. unfold existsb in HSp. rewrite orb_false_r in HSp.
@@ -7113,12 +7155,12 @@ Proof.
 
         apply BITVECTOR_LIST.bv_eq_reflect in HSp.
 
-        unfold get_type' in H4. unfold v_type in H4.
+        unfold get_type' in H2. unfold v_type in H2.
         case_eq (t_interp .[ a1']).
-          intros v_typea1 v_vala1 Htia1. rewrite Htia1 in H4.
+          intros v_typea1 v_vala1 Htia1. rewrite Htia1 in H2.
         rewrite Atom.t_interp_wf in Htia1; trivial.
         unfold apply_binop.
-        apply Typ.eqb_spec in H4.
+        apply Typ.eqb_spec in H2.
 
         (** case a1 = a1' **)
         rewrite eqb_spec in Heq7; rewrite Heq7 in *.
@@ -7136,37 +7178,50 @@ Proof.
           rewrite Htia. easy.
         }
 
-        rewrite H2. rewrite Heq6. simpl.
+        rewrite H0. rewrite Heq6. simpl.
         unfold interp_bv. unfold apply_unop.
 
         rewrite !Atom.t_interp_wf; trivial.
 
-        revert v_vala1 Htia1. rewrite H4.
+        revert v_vala1 Htia1. rewrite H2.
         intros v_vala1 Htia1.
         rewrite Htia1.
         rewrite !Typ.cast_refl.
         unfold Bval.
 
-        assert (H100: (N.of_nat (Datatypes.length (map (Lit.interp rho) bsres))) = (j - i)%N).
+        assert (H100: (N.of_nat (Datatypes.length (map (Lit.interp rho) bsres))) = n0%N).
         {
-           rewrite andb_true_iff in Heq8.
-           destruct Heq8 as (Heq8a, Heq8b).
+           rewrite !andb_true_iff in Heq8.
+           destruct Heq8 as ((Heq8a, Heq8b), Heq8c).
            rewrite map_length.
-           specialize (@extract_interp_main bs1 bsres n i j H0 H1).
+           specialize (@extract_interp_main bs1 bsres i n0 Heq8a).
            intros.
-           apply H6 in Heq8a.
-           unfold RAWBITVECTOR_LIST.bv_extr in Heq8a.
+           unfold RAWBITVECTOR_LIST.bv_extr in H4.
            assert (length (RAWBITVECTOR_LIST.extract (map (Lit.interp rho) bs1) (N.to_nat i)
-           (N.to_nat j)) = length (map (Lit.interp rho) bsres)).
-           { now rewrite Heq8a. }
-           rewrite RAWBITVECTOR_LIST.length_extract, map_length in H7.
-           apply (f_equal (N.of_nat)) in H7.
-           now rewrite N2Nat.id in H7.
-           
+           (N.to_nat (n0 + i))) = length (map (Lit.interp rho) bsres)).
            rewrite N.eqb_eq in Heq8b.
-           rewrite map_length, Heq8b.
-           easy. easy.
-        }
+           rewrite Heq8b in H4.
+           case_eq ((n1 <? n0 + i)%N); intros.
+           apply N.leb_le in Heq8c.
+           assert ((n0 + i <= n1)%N -> (n1 >= n0 + i)%N).
+           { lia. } apply H6 in Heq8c.
+           apply not_ltb2 in Heq8c. 
+           rewrite Heq8c in H5. now contradict H5.
+           rewrite H5 in H4.
+           now rewrite H4.
+           rewrite RAWBITVECTOR_LIST.length_extract, !map_length in H5.
+           assert ((n0 + i - i)%N = n0).
+           { lia. } rewrite H6 in H5.
+           now rewrite <- H5, N2Nat.id.
+           
+           rewrite map_length. 
+           rewrite N.eqb_eq in Heq8b.
+           rewrite Heq8b. unfold is_true.
+           apply N.leb_le in Heq8c.
+           assert ((n0 + i <= n1)%N -> (n1 >= n0 + i)%N).
+           { lia. } now apply H6 in Heq8c.
+           lia.
+         }
 
         unfold BITVECTOR_LIST.of_bits, RAWBITVECTOR_LIST.of_bits.
 
@@ -7189,17 +7244,16 @@ Proof.
           rewrite Htia1. easy.
         }
 
-        rewrite H6 in HSp.
+        rewrite H4 in HSp.
         unfold interp_bv in HSp.
         rewrite Htia1 in HSp.
         unfold interp_bv in HSp. 
 
         revert HSp.
 
-        assert (H101: (N.of_nat (Datatypes.length (map (Lit.interp rho) bs1))) = n).
-        {
-           rewrite andb_true_iff in Heq8.
-           destruct Heq8 as (Heq8a, Heq8b).
+        assert (H101: (N.of_nat (Datatypes.length (map (Lit.interp rho) bs1))) = n1).
+        {  rewrite !andb_true_iff in Heq8.
+           destruct Heq8 as ((Heq8a, Heq8b), Heq8c).
            rewrite map_length.
            now rewrite N.eqb_eq in Heq8b.
         }
@@ -7215,10 +7269,13 @@ Proof.
         rewrite HSp. simpl.
         unfold BITVECTOR_LIST.bv_extr.
         apply eq_rec. simpl.
-        rewrite andb_true_iff in Heq8.
+        rewrite !andb_true_iff in Heq8.
         destruct Heq8 as (Heq8a, Heq8b).
-        now apply extract_interp_main.
-Qed.
+        specialize (@extract_interp_main bs1 bsres i n0).
+        intros.
+        rewrite map_length in H101.
+        rewrite H101 in H5. now apply H5.
+Admitted.
 
 Lemma zextend_interp_zero: forall a, RAWBITVECTOR_LIST.zextend (map (Lit.interp rho) a) O =
 (map (Lit.interp rho) (zextend_lit a 0)).
