src/SMT_terms.v
@@ -773,7 +773,8 @@ Module Atom.
    | UO_BVbitOf (_: N) (_: nat)
    | UO_BVnot   (_: N)
    | UO_BVneg   (_: N)
-   | UO_BVextr  (n: N) (i: N) (j: N) (H0: (n >= j)%N) (H1: (j >= i)%N)
+   | UO_BVextr  (i: N) (n0: N) (n1: N)
+ (*  | UO_BVextr  (n: N) (i: N) (j: N) (H0: (n >= j)%N) (H1: (j >= i)%N) *)
    | UO_BVzextn (n: N) (i: N)
    | UO_BVsextn (n: N) (i: N).
 
@@ -837,7 +838,7 @@ Module Atom.
    | UO_BVbitOf s1 n, UO_BVbitOf s2 m => Nat_eqb n m && N.eqb s1 s2
    | UO_BVnot s1, UO_BVnot s2 => N.eqb s1 s2
    | UO_BVneg s1, UO_BVneg s2 => N.eqb s1 s2
-   | UO_BVextr s1 i1 j1 _ _, UO_BVextr s2 i2 j2 _ _ => N.eqb s1 s2 && N.eqb i1 i2 && N.eqb j1 j2
+   | UO_BVextr i0 n00 n01, UO_BVextr i1 n10 n11 => N.eqb i0 i1 && N.eqb n00 n10 && N.eqb n01 n11
    | UO_BVzextn s1 i1, UO_BVzextn s2 i2 => N.eqb s1 s2 && N.eqb i1 i2
    | UO_BVsextn s1 i1, UO_BVsextn s2 i2 => N.eqb s1 s2 && N.eqb i1 i2
    | _,_ => false
@@ -935,8 +936,7 @@ Module Atom.
       destruct H as ((Ha, Hb), Hc).
       rewrite N.eqb_eq in Ha, Hb, Hc.
       subst.
-      rewrite (proof_irrelevance H0 H2).
-      rewrite (proof_irrelevance H1 H3). reflexivity.
+      reflexivity.
     - intros. apply iff_reflect. split; intros.
       + rewrite !andb_true_iff. inversion H.
         split; try split; try now rewrite N.eqb_eq.
@@ -1097,7 +1097,7 @@ Qed.
         | UO_BVbitOf s _ => (Typ.TBV s, Typ.Tbool)
         | UO_BVnot s => (Typ.TBV s, Typ.TBV s)
         | UO_BVneg s => (Typ.TBV s, Typ.TBV s)
-        | UO_BVextr s i j H0 H1 => (Typ.TBV s, Typ.TBV (j - i))
+        | UO_BVextr i n0 n1 => (Typ.TBV n1, Typ.TBV n0)
         | UO_BVzextn s i => (Typ.TBV s, Typ.TBV (i + s))
         | UO_BVsextn s i => (Typ.TBV s, Typ.TBV (i + s))
         end.
@@ -1278,12 +1278,12 @@ Qed.
            left. exists (Typ.TBV n). now rewrite N.eqb_refl; easy.
            right. intros. rewrite andb_false_r. easy. 
            
-         (case (Typ.eqb (get_type h) (Typ.TBV n))).
-           left. exists (Typ.TBV (j - i)). now rewrite N.eqb_refl; easy.
+         (case (Typ.eqb (get_type h) (Typ.TBV n1))).
+           left. exists (Typ.TBV n0). now rewrite N.eqb_refl; easy.
            right. intros. rewrite andb_false_r. easy. 
            
-         (case (Typ.eqb (get_type h) (Typ.TBV n))).
-           left. exists (Typ.TBV (j - i)). now rewrite N.eqb_refl; easy.
+         (case (Typ.eqb (get_type h) (Typ.TBV n1))).
+           left. exists (Typ.TBV n0). now rewrite N.eqb_refl; easy.
            right. intros. rewrite andb_false_r. easy.
 
          (case (Typ.eqb (get_type h) (Typ.TBV n))).
@@ -1503,8 +1503,8 @@ Qed.
         | UO_BVbitOf s n => apply_unop (Typ.TBV s) Typ.Tbool (BITVECTOR_LIST.bitOf n)
         | UO_BVnot s => apply_unop (Typ.TBV s) (Typ.TBV s) (@BITVECTOR_LIST.bv_not s)
         | UO_BVneg s => apply_unop (Typ.TBV s) (Typ.TBV s) (@BITVECTOR_LIST.bv_neg s)
-        | UO_BVextr s i j H0 H1 => 
-          apply_unop (Typ.TBV s) (Typ.TBV (j - i)) (@BITVECTOR_LIST.bv_extr s i j H0 H1)
+        | UO_BVextr i n0 n1 => 
+          apply_unop (Typ.TBV n1) (Typ.TBV n0) (@BITVECTOR_LIST.bv_extr i n0 n1)
         | UO_BVzextn s i => 
           apply_unop (Typ.TBV s) (Typ.TBV (i + s)) (@BITVECTOR_LIST.bv_zextn s i)
         | UO_BVsextn s i => 
@@ -1747,7 +1747,7 @@ Qed.
         apply Typ.eqb_spec in Hb.
         revert x y Hx Hy.
         rewrite Hb. intros.
-        exists (@BITVECTOR_LIST.bv_extr n i j H0 H1 y); auto. rewrite Typ.cast_refl; auto.
+        exists (@BITVECTOR_LIST.bv_extr i n0 n1 y); auto. rewrite Typ.cast_refl; auto.
         (* bv_zextn *)
         intros.
         apply andb_true_iff in H. destruct H as (Ha, Hb).
@@ -2043,7 +2043,7 @@ Qed.
               rewrite N.eqb_refl in H. now contradict H.
               now rewrite H.
             (* bv_extr *)
-            specialize (H (Typ.TBV (j - i))). simpl in H. rewrite andb_false_iff in H.
+            specialize (H (Typ.TBV n0)). simpl in H. rewrite andb_false_iff in H.
             destruct H as [ H | H].
               rewrite N.eqb_refl in H. now contradict H.
               now rewrite H.
@@ -2372,8 +2372,8 @@ Qed.
         case (Typ.cast (v_type Typ.type interp_t (a .[ i])) (Typ.TBV n)); simpl; [ | exists true; auto]. intro k; exists (BITVECTOR_LIST.bitOf n0 (k interp_t x)) ; auto.
         case (Typ.cast (v_type Typ.type interp_t (a .[ i])) (Typ.TBV n)); simpl; [ | exists true; auto]. intro k; exists (BITVECTOR_LIST.bv_not (k interp_t x)) ; auto.
         case (Typ.cast (v_type Typ.type interp_t (a .[ i])) (Typ.TBV n)); simpl; [ | exists true; auto]. intro k; exists (BITVECTOR_LIST.bv_neg (k interp_t x)) ; auto.
-        case (Typ.cast (v_type Typ.type interp_t (a .[ i])) (Typ.TBV n)); 
-        simpl; [ | exists true; auto]. intro k; exists (BITVECTOR_LIST.bv_extr H0 H1 (k interp_t x)) ; auto.
+        case (Typ.cast (v_type Typ.type interp_t (a .[ i])) (Typ.TBV n1));
+        simpl; [ | exists true; auto]. intro k; exists (BITVECTOR_LIST.bv_extr i0 n0 (k interp_t x)) ; auto.
         case (Typ.cast (v_type Typ.type interp_t (a .[ i])) (Typ.TBV n)); 
         simpl; [ | exists true; auto]. intro k. exists (BITVECTOR_LIST.bv_zextn i0 (k interp_t x)) ; auto.
         case (Typ.cast (v_type Typ.type interp_t (a .[ i])) (Typ.TBV n)); 
